parsing/PEG_CFGScript.sml
@@ -169,7 +169,21 @@ val peg_eval_LetDec_wrongtok = store_thm(
        peg_TypeDec_def, peg_eval_seq_SOME, tokeq_def, peg_eval_tok_SOME,
        peg_eval_choicel_CONS, peg_eval_seql_CONS]);
 
-fun print_tac s g = (print ("print_tac: "^s^"\n"); ALL_TAC g)
+val peg_eval_rpt_never_NONE = store_thm(
+  "peg_eval_rpt_never_NONE",
+  ``¬peg_eval G (i, rpt sym f) NONE``,
+  simp[Once pegTheory.peg_eval_cases]);
+val _ = export_rewrites ["peg_eval_rpt_never_NONE"]
+
+fun print_tac s (g as (asl,w)) = let
+  fun mmlnt_test t = is_const t andalso type_of t = ``:MMLnonT``
+in
+  case get_first (Lib.total (find_term mmlnt_test)) asl of
+      NONE => raise Fail "No MMLnonT in goal"
+    | SOME t => if term_to_string t = s then
+                  (print ("print_tac: "^s^"\n"); ALL_TAC g)
+                else raise Fail ("MMLnonT not "^s)
+end
 
 val pegsym_to_sym_def = Define`
   (pegsym_to_sym (tok P f) = if f = mktokLf then { TK t | P t } else ∅) ∧
@@ -245,12 +259,23 @@ val peg_linfix_correct_lemma = store_thm(
     by fs[SUBSET_DEF] >>
   simp[]);
 
+val length_no_greater = store_thm(
+  "length_no_greater",
+  ``peg_eval G (i0, sym) (SOME(i,r)) ⇒ LENGTH i ≤ LENGTH i0``,
+  metis_tac[pegTheory.peg_eval_suffix',
+            DECIDE ``x ≤ y:num ⇔ x < y ∨ x = y``]);
+
 val _ = augment_srw_ss [rewrites [
   peg_eval_seql_CONS, peg_eval_tok_SOME, tokeq_def, bindNT_def, mktokLf_def,
   peg_eval_choicel_CONS, pegf_def, peg_eval_seq_SOME, pnt_def, peg_eval_try,
   try_def]]
 
-(*
+val peg_eval_nTyOp_wrongtok = store_thm(
+  "peg_eval_nTyOp_wrongtok",
+  ``¬peg_eval mmlPEG (LparT::i, nt (mkNT nTyOp) f) (SOME x)``,
+  simp[Once pegTheory.peg_eval_cases, mmlpeg_rules_applied, FDOM_cmlPEG] >>
+  simp[Once pegTheory.peg_eval_cases, mmlpeg_rules_applied, FDOM_cmlPEG]);
+
 val peg_correct = store_thm(
   "peg_correct",
   ``∀N i0 s i pts.
@@ -566,21 +591,287 @@ val peg_correct = store_thm(
             first_assum (mp_tac o PART_MATCH (lhand o rand) patth o concl)) >>
           simp[NT_rank_def] >> strip_tac >> rveq >> simp[]) >>
       asm_match `isLongidT h` >> Cases_on `h` >> fs[])
-  >- (print_tac "nDType" >> simp[peg_DType_def, peg_eval_choice] >>
-      strip_tac >> rveq >> simp[sumID_def] >>
+  >- (print_tac "nTypeList1" >> strip_tac >> rveq >>
+      dsimp[cmlG_FDOM, cmlG_applied, listTheory.APPEND_EQ_CONS, MAP_EQ_SING] >>
+      csimp[] >>
+      `NT_rank (mkNT nType) < NT_rank (mkNT nTypeList1)` by simp[NT_rank_def]
+      >- (first_x_assum (erule mp_tac) >>
+          erule assume_tac
+                (length_no_greater |> Q.GEN `sym`
+                                   |> Q.ISPEC `nt (mkNT nType) I` |> GEN_ALL) >>
+          first_x_assum (fn patth =>
+            first_assum (mp_tac o PART_MATCH (lhand o rand) patth o concl)) >>
+          fs[] >> asimp[] >> rpt strip_tac >> rveq >> simp[])
+      >- (first_x_assum (erule strip_assume_tac) >> rveq >> simp[]) >>
+      first_x_assum (erule strip_assume_tac) >> rveq >> simp[])
+  >- (print_tac "nTypeList2" >> strip_tac >> rveq >>
+      dsimp[cmlG_applied, cmlG_FDOM, listTheory.APPEND_EQ_CONS, MAP_EQ_SING]>>
+      csimp[] >>
+      `NT_rank (mkNT nType) < NT_rank (mkNT nTypeList2)` by simp[NT_rank_def]>>
+      first_x_assum (erule strip_assume_tac) >> rveq >> simp[] >>
+      first_x_assum (fn patth =>
+            first_assum (mp_tac o PART_MATCH (lhand o rand) patth o concl)) >>
+      erule assume_tac
+            (length_no_greater |> Q.GEN `sym` |> Q.ISPEC `nt (mkNT nType) I`
+                               |> GEN_ALL) >> fs[] >> asimp[] >>
+      strip_tac >> rveq >> simp[])
+  >- (print_tac "nDType" >> strip_tac >> rveq >> simp[]
       >- (qpat_assum `peg_eval mmlPEG (i1, rpt X Y) Z` mp_tac >>
-          dsimp[peg_eval_rpt] >> qx_gen_tac `tyops` >> strip_tac >> rveq >>
+          simp[peg_eval_rpt] >>
+          disch_then (qxchl [`tyops`] strip_assume_tac) >> rveq >> simp[] >>
           asm_match `peg_eval_list mmlPEG (i1, nt (mkNT nTyOp) I) (i,tyops)`>>
           pop_assum mp_tac >>
           `∃i2. LENGTH i2 < SUC (LENGTH i1) ∧ i1 = i2` by simp[] >>
           pop_assum SUBST1_TAC >> pop_assum mp_tac >>
-          map_every qid_spec_tac [`i2`, `i`, `tyops`] >> Induct
+          asm_match `isTyvarT tyv` >>
+          `∃acc.
+             MAP ptree_head acc ∈ mmlG.rules ' (mkNT nDType) ∧
+             (∀pt. MEM pt acc ⇒ valid_ptree mmlG pt) ∧
+             TK tyv::MAP TK i2 = FLAT (MAP ptree_fringe acc) ++ MAP TK i2 ∧
+             [Lf (TK tyv)] = acc`
+            by (simp[cmlG_FDOM, cmlG_applied] >> Cases_on `tyv` >> fs[]) >>
+          ntac 2 (pop_assum SUBST1_TAC) >> ntac 2 (pop_assum mp_tac) >>
+          map_every qid_spec_tac [`acc`, `i2`, `i`, `tyops`] >> Induct
           >- (simp[Once pegTheory.peg_eval_cases] >>
-              simp[cmlG_FDOM, cmlG_applied] >> asm_match `isTyvarT t` >>
-              Cases_on `t` >> fs[]) >>
-          simp[Once pegTheory.peg_eval_cases] >> rpt strip_tac >>
-          fs[] >> first_x_assum (erule strip_assume_tac) >> rveq >>
-          simp[]
+              simp[cmlG_FDOM, cmlG_applied]) >>
+          map_every qx_gen_tac [`tyop`, `i`, `i2`, `acc`] >>
+          simp[Once pegTheory.peg_eval_cases] >> ntac 3 strip_tac >>
+          disch_then (qxchl [`i3`] strip_assume_tac) >>
+          fs[] >> first_x_assum (erule mp_tac) >>
+          disch_then (qxchl [`tyop_pt`] strip_assume_tac) >> rveq >>
+          simp[] >>
+          `LENGTH i3 < LENGTH i2`
+            by metis_tac[not_peg0_LENGTH_decreases, peg0_nTyOp] >>
+          `LENGTH i3 < SUC (LENGTH i1)` by decide_tac >>
+          first_x_assum
+            (qspecl_then [`i`, `i3`, `[Nd (mkNT nDType) acc; tyop_pt]`]
+                         mp_tac)>>
+          simp[cmlG_applied, cmlG_FDOM, DISJ_IMP_THM, FORALL_AND_THM])
+      >- (`NT_rank (mkNT nTyOp) < NT_rank (mkNT nDType)` by simp[NT_rank_def] >>
+          first_x_assum (erule mp_tac) >>
+          disch_then (qxchl [`tyop_pt`] strip_assume_tac) >> rveq >> simp[] >>
+          qpat_assum `peg_eval mmlPEG XX NONE` (K ALL_TAC) >>
+          erule strip_assume_tac
+            (MATCH_MP not_peg0_LENGTH_decreases peg0_nTyOp) >>
+          qpat_assum `peg_eval mmlPEG (II, rpt XX FF) YY` mp_tac >>
+          simp[peg_eval_rpt] >> disch_then (qxchl [`tyops`] strip_assume_tac) >>
+          rveq >> simp[] >>
+          asm_match `peg_eval_list mmlPEG (i1, nt (mkNT nTyOp) I) (i,tyops)`>>
+          pop_assum mp_tac >>
+          `∃i2. LENGTH i2 < LENGTH i0 ∧ i1 = i2` by simp[] >>
+          pop_assum SUBST1_TAC >> pop_assum mp_tac >>
+          `∃acc.
+             MAP ptree_head acc ∈ mmlG.rules ' (mkNT nDType) ∧
+             (∀pt. MEM pt acc ⇒ valid_ptree mmlG pt) ∧
+             ptree_fringe tyop_pt ++ MAP TK i2 =
+               FLAT (MAP ptree_fringe acc) ++ MAP TK i2 ∧
+             [tyop_pt] = acc`
+            by (simp[cmlG_FDOM, cmlG_applied]) >>
+          ntac 2 (pop_assum SUBST1_TAC) >> ntac 2 (pop_assum mp_tac) >>
+          map_every qid_spec_tac [`acc`, `i2`, `i`, `tyops`] >> Induct
+          >- (simp[Once pegTheory.peg_eval_cases] >>
+              simp[cmlG_FDOM, cmlG_applied]) >>
+          map_every qx_gen_tac [`tyop`, `i`, `i2`, `acc`] >>
+          simp[Once pegTheory.peg_eval_cases] >> ntac 3 strip_tac >>
+          disch_then (qxchl [`i3`] strip_assume_tac) >>
+          first_x_assum (erule mp_tac) >>
+          disch_then (qxchl [`tyop_pt2`] strip_assume_tac) >> rveq >>
+          simp[] >>
+          `LENGTH i3 < LENGTH i2`
+            by metis_tac[not_peg0_LENGTH_decreases, peg0_nTyOp] >>
+          `LENGTH i3 < LENGTH i0` by decide_tac >>
+          first_x_assum
+            (qspecl_then [`i`, `i3`, `[Nd (mkNT nDType) acc; tyop_pt2]`]
+                         mp_tac)>>
+          simp[cmlG_applied, cmlG_FDOM, DISJ_IMP_THM, FORALL_AND_THM])
+      >- ((* type in parentheses followed by tyops case *)
+          rpt (qpat_assum `peg_eval mmlPEG XX NONE` (K ALL_TAC)) >>
+          asm_match
+            `peg_eval mmlPEG (i0,nt (mkNT nType) I) (SOME(RparT::i1,r))`>>
+          loseC ``NT_rank`` >>
+          first_assum (fn patth =>
+            first_assum (mp_tac o PART_MATCH (lhand o rand) patth o concl)) >>
+          simp_tac(srw_ss()) [] >> ASM_REWRITE_TAC[] >>
+          disch_then (qxchl [`type_pt`] strip_assume_tac) >> rveq >> simp[] >>
+          erule mp_tac
+            (length_no_greater |> Q.GEN `sym` |> Q.ISPEC `nt (mkNT nType) I`
+                               |> GEN_ALL) >> simp[] >> strip_tac >>
+          fs[] >> `LENGTH i1 < SUC (LENGTH i0)` by decide_tac >>
+          qpat_assum `peg_eval mmlPEG (II, rpt XX FF) YY` mp_tac >>
+          simp[peg_eval_rpt] >> disch_then (qxchl [`tyops`] strip_assume_tac) >>
+          rveq >> simp[] >>
+          asm_match `peg_eval_list mmlPEG (i1, nt (mkNT nTyOp) I) (i,tyops)`>>
+          pop_assum mp_tac >>
+          `∃i2. LENGTH i2 < SUC (LENGTH i0) ∧ i1 = i2` by simp[] >>
+          pop_assum SUBST1_TAC >> pop_assum mp_tac >>
+          `∃acc.
+             MAP ptree_head acc ∈ mmlG.rules ' (mkNT nDType) ∧
+             (∀pt. MEM pt acc ⇒ valid_ptree mmlG pt) ∧
+             TK LparT::(ptree_fringe type_pt ++ [TK RparT] ++ MAP TK i2) =
+               FLAT (MAP ptree_fringe acc) ++ MAP TK i2 ∧
+             [Lf (TK LparT); type_pt; Lf (TK RparT)] = acc`
+            by simp[cmlG_FDOM, cmlG_applied, DISJ_IMP_THM, FORALL_AND_THM] >>
+          ntac 2 (pop_assum SUBST1_TAC) >> ntac 2 (pop_assum mp_tac) >>
+          map_every qid_spec_tac [`acc`, `i2`, `i`, `tyops`] >> Induct
+          >- (simp[Once pegTheory.peg_eval_cases] >>
+              simp[cmlG_FDOM, cmlG_applied]) >>
+          map_every qx_gen_tac [`tyop`, `i`, `i2`, `acc`] >>
+          simp[Once pegTheory.peg_eval_cases] >> ntac 3 strip_tac >>
+          disch_then (qxchl [`i3`] strip_assume_tac) >>
+          first_x_assum (erule mp_tac) >>
+          disch_then (qxchl [`tyop_pt`] strip_assume_tac) >> rveq >>
+          simp[] >>
+          `LENGTH i3 < LENGTH i2`
+            by metis_tac[not_peg0_LENGTH_decreases, peg0_nTyOp] >>
+          `LENGTH i3 < SUC(LENGTH i0)` by decide_tac >>
+          first_x_assum
+            (qspecl_then [`i`, `i3`, `[Nd (mkNT nDType) acc; tyop_pt]`]
+                         mp_tac)>>
+          simp[cmlG_applied, cmlG_FDOM, DISJ_IMP_THM, FORALL_AND_THM]) >>
+        (* tuple followed by at least one tyop case *)
+        rpt (qpat_assum `peg_eval GG XX NONE` (K ALL_TAC)) >>
+        loseC ``NT_rank`` >>
+        asm_match `peg_eval mmlPEG (i1, nt (mkNT nTypeList2) I)
+                      (SOME (RparT::i2, r))` >> fs[] >>
+        first_assum (fn patth =>
+          first_assum (mp_tac o PART_MATCH (lhand o rand) patth o
+                       assert (free_in ``nTypeList2``) o concl)) >>
+        simp_tac(srw_ss())[] >> ASM_REWRITE_TAC[] >>
+        disch_then (qxchl [`tyl2_pt`] strip_assume_tac) >> rveq >> simp[] >>
+        asm_match `peg_eval mmlPEG (i2, nt(mkNT nTyOp) I) (SOME(i3,r))` >>
+        first_assum (mp_tac o MATCH_MP length_no_greater o
+                     assert (free_in ``nTypeList2`` o concl)) >> simp[] >>
+        strip_tac >> `LENGTH i2 < SUC (LENGTH i1)` by decide_tac >>
+        first_assum (erule mp_tac) >>
+        disch_then (qxchl [`tyop_pt`] strip_assume_tac) >> rveq >> simp[]>>
+        first_assum (assume_tac o MATCH_MP length_no_greater o
+                     assert (free_in ``nTyOp`` o concl) o
+                     assert (free_in ``i2 : token list`` o concl)) >>
+        `LENGTH i3 < SUC (LENGTH i1)` by decide_tac >>
+        qpat_assum `peg_eval mmlPEG (II, rpt XX FF) YY` mp_tac >>
+        simp[peg_eval_rpt] >> disch_then (qxchl [`tyops`] strip_assume_tac) >>
+        rveq >> simp[] >>
+        asm_match `peg_eval_list mmlPEG (i3, nt (mkNT nTyOp) I) (i,tyops)`>>
+        pop_assum mp_tac >>
+        `∃i4. LENGTH i4 < SUC (LENGTH i1) ∧ i3 = i4` by simp[] >>
+        pop_assum SUBST1_TAC >> pop_assum mp_tac >>
+        `∃acc.
+           MAP ptree_head acc ∈ mmlG.rules ' (mkNT nDType) ∧
+           (∀pt. MEM pt acc ⇒ valid_ptree mmlG pt) ∧
+           TK LparT::(ptree_fringe tyl2_pt ++ [TK RparT] ++
+                      ptree_fringe tyop_pt ++ MAP TK i4) =
+             FLAT (MAP ptree_fringe acc) ++ MAP TK i4 ∧
+           [Lf (TK LparT); tyl2_pt; Lf (TK RparT); tyop_pt] = acc`
+          by simp[cmlG_FDOM, cmlG_applied, DISJ_IMP_THM, FORALL_AND_THM] >>
+        ntac 2 (pop_assum SUBST1_TAC) >> ntac 2 (pop_assum mp_tac) >>
+        map_every qid_spec_tac [`acc`, `i4`, `i`, `tyops`] >> Induct
+        >- (simp[Once pegTheory.peg_eval_cases] >>
+            simp[cmlG_FDOM, cmlG_applied]) >>
+        map_every qx_gen_tac [`tyop`, `i`, `i4`, `acc`] >>
+        simp[Once pegTheory.peg_eval_cases] >> ntac 3 strip_tac >>
+        disch_then (qxchl [`i5`] strip_assume_tac) >>
+        first_x_assum (erule mp_tac) >>
+        disch_then (qxchl [`tyop_pt2`] strip_assume_tac) >> rveq >>
+        simp[] >>
+        `LENGTH i5 < LENGTH i4`
+          by metis_tac[not_peg0_LENGTH_decreases, peg0_nTyOp] >>
+        `LENGTH i5 < SUC(LENGTH i1)` by decide_tac >>
+        first_x_assum
+          (qspecl_then [`i`, `i5`, `[Nd (mkNT nDType) acc; tyop_pt2]`]
+                       mp_tac)>>
+        simp[cmlG_applied, cmlG_FDOM, DISJ_IMP_THM, FORALL_AND_THM])
+  >- (print_tac "nType" >> simp[peg_Type_def, peg_eval_choice, sumID_def] >>
+      `NT_rank (mkNT nDType) < NT_rank (mkNT nType)` by simp[NT_rank_def] >>
+      strip_tac >> rveq >> simp[]
+      >- (first_x_assum (erule strip_assume_tac) >> rveq >> simp[] >>
+          first_assum (assume_tac o MATCH_MP length_no_greater o
+                       assert (free_in ``nDType`` o concl)) >> fs[] >>
+          first_x_assum (fn patth =>
+            first_assum (mp_tac o PART_MATCH (lhand o rand) patth o
+                         assert (free_in ``nType``) o concl)) >>
+          asimp[] >> strip_tac >> rveq >> dsimp[cmlG_FDOM, cmlG_applied]) >>
+      first_x_assum (erule strip_assume_tac) >> rveq >>
+      dsimp[cmlG_applied, cmlG_FDOM])
+  >- (print_tac "nFDecl" >> strip_tac >> rveq >> simp[] >>
+      `NT_rank (mkNT nV) < NT_rank (mkNT nFDecl)` by simp[NT_rank_def] >>
+      first_x_assum (erule strip_assume_tac) >> rveq >> simp[] >>
+      erule assume_tac
+        (MATCH_MP not_peg0_LENGTH_decreases peg0_nV |> GEN_ALL) >>
+      first_assum (erule strip_assume_tac) >> rveq >> dsimp[] >>
+      first_assum (assume_tac o MATCH_MP length_no_greater o
+                   assert (free_in ``nVlist1`` o concl)) >> fs[] >>
+      first_x_assum (fn patth =>
+            first_assum (mp_tac o PART_MATCH (lhand o rand) patth o
+                         assert (free_in ``nE``) o concl)) >>
+      asimp[] >> strip_tac >> rveq >> simp[cmlG_FDOM, cmlG_applied])
+  >- (print_tac "nAndFDecls" >>
+      disch_then (match_mp_tac o MATCH_MP peg_linfix_correct_lemma) >>
+      simp[SUBSET_DEF, pegsym_to_sym_def, DISJ_IMP_THM, FORALL_AND_THM,
+           cmlG_applied, cmlG_FDOM] >> first_x_assum match_mp_tac >>
+      simp[NT_rank_def])
+  >- (print_tac "nPE'" >> strip_tac >> rveq >> simp[] >>
+      `NT_rank (mkNT nPattern) < NT_rank (mkNT nPE')` by simp[NT_rank_def] >>
+      first_x_assum (erule strip_assume_tac) >> rveq >> simp[] >>
+      first_assum (assume_tac o MATCH_MP length_no_greater o
+                   assert (free_in ``nPattern`` o concl)) >> fs[] >>
+      first_x_assum (fn patth =>
+            first_assum (mp_tac o PART_MATCH (lhand o rand) patth o
+                         assert (free_in ``nE'``) o concl)) >>
+      asimp[] >> strip_tac >> rveq >> dsimp[cmlG_FDOM, cmlG_applied])
+  >- (print_tac "nPE" >> strip_tac >> rveq >> simp[] >>
+      `NT_rank (mkNT nPattern) < NT_rank (mkNT nPE)` by simp[NT_rank_def] >>
+      first_x_assum (erule strip_assume_tac) >> rveq >> simp[] >>
+      first_assum (assume_tac o MATCH_MP length_no_greater o
+                   assert (free_in ``nPattern`` o concl)) >> fs[] >>
+      first_x_assum (fn patth =>
+            first_assum (mp_tac o PART_MATCH (lhand o rand) patth o
+                         assert (free_in ``nE``) o concl)) >>
+      asimp[] >> strip_tac >> rveq >> dsimp[cmlG_FDOM, cmlG_applied])
+  >- (print_tac "nPEs" >>
+      `NT_rank (mkNT nPE') < NT_rank (mkNT nPEs) ∧
+       NT_rank (mkNT nPE) < NT_rank (mkNT nPEs)`
+         by simp[NT_rank_def] >>
+      strip_tac >> rveq >> simp[] >> first_x_assum (erule strip_assume_tac) >>
+      rveq >> simp[cmlG_applied, cmlG_FDOM] >>
+      first_assum (assume_tac o MATCH_MP length_no_greater o
+                   assert (free_in ``nPE'`` o concl)) >> fs[] >>
+      first_x_assum (fn patth =>
+            first_assum (mp_tac o PART_MATCH (lhand o rand) patth o
+                         assert (free_in ``nPEs``) o concl)) >>
+      asimp[] >> strip_tac >> rveq >> dsimp[])
+  >- (print_tac "nE'" >> strip_tac >> rveq >> simp[]
+      >- ((* raise case *)
+          loseC ``NT_rank`` >>
+          first_x_assum (fn patth =>
+            first_assum (mp_tac o PART_MATCH (lhand o rand) patth o concl)) >>
+          simp[] >> strip_tac >> rveq >> dsimp[cmlG_FDOM, cmlG_applied])
+      >- ((* Ehandle' case *)
+          loseC ``LENGTH`` >>
+          first_x_assum (fn patth =>
+            first_assum (mp_tac o PART_MATCH (lhand o rand) patth o concl)) >>
+          simp[NT_rank_def] >> strip_tac >> rveq >>
+          dsimp[cmlG_FDOM, cmlG_applied])
+      >- ((* if-then-else case *) loseC ``NT_rank`` >>
+          first_assum (fn patth =>
+            first_assum (mp_tac o PART_MATCH (lhand o rand) patth o
+                         assert (free_in ``ThenT``) o concl)) >>
+          simp_tac (srw_ss())[] >> ASM_REWRITE_TAC[] >>
+          strip_tac >> rveq >> simp[]
+          first_assum (fn patth =>
+            first_assum (mp_tac o PART_MATCH (lhand o rand) patth o
+                         assert (free_in ``ElseT``) o concl)) >>
+          simp_tac (srw_ss())[] >> ASM_REWRITE_TAC[] >> asimp[]
+
+
+
+
+
+
+
+
+
+
+
 
 
 
